src/dvspec/dafny/att_spec_proofs/ind_inv2.dfy
@@ -75,6 +75,45 @@ module Att_Ind_Inv_With_Empty_Initial_Attestation_Slashing_DB2
         }        
     }
 
+    lemma lemma2_inv_attestation_duty_queue_is_ordered_4_body_body(
+        dvn: DVState, 
+        n: BLSPubkey,
+        n_state: DVCNodeState,
+        n'_state: DVCNodeState,
+        index_next_attestation_duty_to_be_served: nat
+    )
+    requires inv_attestation_duty_queue_is_ordered_4_body_body(dvn, n , n_state, index_next_attestation_duty_to_be_served)
+    requires n_state.attestation_duties_queue == n'_state.attestation_duties_queue
+    ensures inv_attestation_duty_queue_is_ordered_4_body_body(dvn, n , n'_state, index_next_attestation_duty_to_be_served)
+    {
+        if |n_state.attestation_duties_queue| > 0
+        {
+            forall i: nat|
+                inv_attestation_duty_queue_is_ordered_4_body_body_premise(
+                    dvn,
+                    n, 
+                    n'_state,
+                    i,
+                    index_next_attestation_duty_to_be_served
+                )
+            ensures 
+                var last := n_state.attestation_duties_queue[|n_state.attestation_duties_queue|-1];
+                last.slot == dvn.sequence_attestation_duties_to_be_served[i].attestation_duty.slot         
+        
+            {
+
+                assert inv_attestation_duty_queue_is_ordered_4_body_body_premise(
+                    dvn,
+                    n, 
+                    n_state,
+                    i,
+                    index_next_attestation_duty_to_be_served                     
+                );
+            }  
+        }
+      
+    }    
+
     lemma lemma3_inv_attestation_duty_queue_is_ordered_3_body_body(
         dvn: DVState, 
         n: BLSPubkey,
@@ -116,6 +155,44 @@ module Att_Ind_Inv_With_Empty_Initial_Attestation_Slashing_DB2
             );
         }         
     }
+
+    lemma lemma3_inv_attestation_duty_queue_is_ordered_4_body_body(
+        dvn: DVState, 
+        n: BLSPubkey,
+        n_state: DVCNodeState,
+        n'_state: DVCNodeState,
+        index_next_attestation_duty_to_be_served: nat
+    )
+    requires inv_attestation_duty_queue_is_ordered_4_body_body(dvn, n , n_state, index_next_attestation_duty_to_be_served)
+    requires |n_state.attestation_duties_queue| > 0
+    requires  n'_state.attestation_duties_queue == n_state.attestation_duties_queue[1..]
+    requires inv_attestation_duty_queue_is_ordered_4_body_body(dvn, n , n_state, index_next_attestation_duty_to_be_served)
+    {
+        if |n'_state.attestation_duties_queue| > 0
+        {
+            forall i: nat  |
+                inv_attestation_duty_queue_is_ordered_4_body_body_premise(
+                    dvn,
+                    n, 
+                    n'_state,
+                    i,
+                    index_next_attestation_duty_to_be_served
+                )
+            ensures 
+                var last := n_state.attestation_duties_queue[|n_state.attestation_duties_queue|-1];
+                    last.slot == dvn.sequence_attestation_duties_to_be_served[i].attestation_duty.slot 
+            {
+                assert inv_attestation_duty_queue_is_ordered_4_body_body_premise(
+                    dvn,
+                    n, 
+                    n_state,
+                    i,
+                    index_next_attestation_duty_to_be_served                     
+                );
+            }    
+        }
+    }
+
 
     lemma  lemma_on_first_seq_element_elimination<T>(
         s1: seq<T>,
@@ -3247,6 +3324,418 @@ module Att_Ind_Inv_With_Empty_Initial_Attestation_Slashing_DB2
                 }   
 
         }
-    }         
+    }    
+
+    lemma lemma_inv_attestation_duty_queue_is_ordered_4_f_serve_attestation_duty(
+        process: DVCNodeState,
+        attestation_duty: AttestationDuty,
+        s': DVCNodeState,
+        dvn: DVState,
+        n: BLSPubkey,
+        index_next_attestation_duty_to_be_served: nat
+    )
+    requires f_serve_attestation_duty.requires(process, attestation_duty)
+    requires s' == f_serve_attestation_duty(process, attestation_duty).state   
+    requires index_next_attestation_duty_to_be_served > 0    
+    // requires inv_attestation_duty_queue_is_ordered_3_body_body(dvn, n, process) 
+    requires inv_attestation_duty_queue_is_ordered_4_body_body(dvn, n, process, index_next_attestation_duty_to_be_served-1)  
+    requires is_sequence_attestation_duties_to_be_served_orderd(dvn);
+    requires 
+                var an' := dvn.sequence_attestation_duties_to_be_served[index_next_attestation_duty_to_be_served-1];
+                && an'.attestation_duty == attestation_duty
+                && an'.node == n
+    ensures inv_attestation_duty_queue_is_ordered_4_body_body(dvn, n, s', index_next_attestation_duty_to_be_served);
+    {
+        var new_p := process.(
+                attestation_duties_queue := process.attestation_duties_queue + [attestation_duty],
+                all_rcvd_duties := process.all_rcvd_duties + {attestation_duty}
+        );
+
+        assert inv_attestation_duty_queue_is_ordered_4_body_body(dvn, n, new_p, index_next_attestation_duty_to_be_served);         
+
+        lemma_inv_attestation_duty_queue_is_ordered_4_f_check_for_next_queued_duty(new_p, s', dvn, n, index_next_attestation_duty_to_be_served);
+    } 
+
+    lemma lemma_inv_attestation_duty_queue_is_ordered_4_f_att_consensus_decided(
+        process: DVCNodeState,
+        id: Slot,
+        decided_attestation_data: AttestationData,        
+        s': DVCNodeState,
+        dvn: DVState,
+        n: BLSPubkey,
+        index_next_attestation_duty_to_be_served: nat        
+    )
+    requires f_att_consensus_decided.requires(process, id, decided_attestation_data)
+    requires s' == f_att_consensus_decided(process, id, decided_attestation_data).state
+    requires inv_attestation_duty_queue_is_ordered_4_body_body(dvn, n, process, index_next_attestation_duty_to_be_served)
+    ensures inv_attestation_duty_queue_is_ordered_4_body_body(dvn, n, s', index_next_attestation_duty_to_be_served); 
+    {
+        // TODO: Remove below by changing spec
+        assume id == process.current_attestation_duty.safe_get().slot;        
+        var local_current_attestation_duty := process.current_attestation_duty.safe_get();
+        var attestation_slashing_db := f_update_attestation_slashing_db(process.attestation_slashing_db, decided_attestation_data);
+
+        var fork_version := bn_get_fork_version(compute_start_slot_at_epoch(decided_attestation_data.target.epoch));
+        var attestation_signing_root := compute_attestation_signing_root(decided_attestation_data, fork_version);
+        var attestation_signature_share := rs_sign_attestation(decided_attestation_data, fork_version, attestation_signing_root, process.rs);
+        var attestation_with_signature_share := AttestationShare(
+                aggregation_bits := get_aggregation_bits(local_current_attestation_duty.validator_index),
+                data := decided_attestation_data, 
+                signature := attestation_signature_share
+            ); 
+
+        var s_mod := 
+            process.(
+                current_attestation_duty := None,
+                attestation_shares_to_broadcast := process.attestation_shares_to_broadcast[local_current_attestation_duty.slot := attestation_with_signature_share],
+                attestation_slashing_db := attestation_slashing_db,
+                attestation_consensus_engine_state := updateConsensusInstanceValidityCheck(
+                    process.attestation_consensus_engine_state,
+                    attestation_slashing_db
+                )
+            );
+
+        lemma2_inv_attestation_duty_queue_is_ordered_4_body_body(dvn, n, process, s_mod, index_next_attestation_duty_to_be_served);
+        lemma_inv_attestation_duty_queue_is_ordered_4_f_check_for_next_queued_duty(s_mod, s', dvn, n, index_next_attestation_duty_to_be_served);             
+    }       
+
+    lemma lemma_inv_attestation_duty_queue_is_ordered_4_f_listen_for_new_imported_blocks(
+        process: DVCNodeState,
+        block: BeaconBlock,
+        s': DVCNodeState,
+        dvn: DVState,
+        n: BLSPubkey,
+        index_next_attestation_duty_to_be_served: nat        
+    )
+    requires f_listen_for_new_imported_blocks.requires(process, block)
+    requires s' == f_listen_for_new_imported_blocks(process, block).state       
+    requires inv_attestation_duty_queue_is_ordered_4_body_body(dvn, n, process, index_next_attestation_duty_to_be_served)
+    ensures inv_attestation_duty_queue_is_ordered_4_body_body(dvn, n, s', index_next_attestation_duty_to_be_served)
+    {
+        var new_consensus_instances_already_decided := f_listen_for_new_imported_blocks_helper_1(process, block);
+
+        var att_consensus_instances_already_decided := process.future_att_consensus_instances_already_decided + new_consensus_instances_already_decided;
+
+        var future_att_consensus_instances_already_decided := 
+            f_listen_for_new_imported_blocks_helper_2(process, att_consensus_instances_already_decided);
+
+        var new_process :=
+                process.(
+                    future_att_consensus_instances_already_decided := future_att_consensus_instances_already_decided,
+                    attestation_consensus_engine_state := stopConsensusInstances(
+                                    process.attestation_consensus_engine_state,
+                                    att_consensus_instances_already_decided.Keys
+                    ),
+                    attestation_shares_to_broadcast := process.attestation_shares_to_broadcast - att_consensus_instances_already_decided.Keys,
+                    rcvd_attestation_shares := process.rcvd_attestation_shares - att_consensus_instances_already_decided.Keys                    
+                );    
+                                 
+
+        if new_process.current_attestation_duty.isPresent() && new_process.current_attestation_duty.safe_get().slot in att_consensus_instances_already_decided
+        {
+            // Stop(current_attestation_duty.safe_get().slot);
+            var decided_attestation_data := att_consensus_instances_already_decided[new_process.current_attestation_duty.safe_get().slot];
+            var new_attestation_slashing_db := f_update_attestation_slashing_db(new_process.attestation_slashing_db, decided_attestation_data);
+            var s_mod := new_process.(
+                current_attestation_duty := None,
+                attestation_slashing_db := new_attestation_slashing_db,
+                attestation_consensus_engine_state := updateConsensusInstanceValidityCheck(
+                    new_process.attestation_consensus_engine_state,
+                    new_attestation_slashing_db
+                )                
+            );
+            
+            lemma2_inv_attestation_duty_queue_is_ordered_4_body_body(dvn, n, process, s_mod, index_next_attestation_duty_to_be_served);
+            lemma_inv_attestation_duty_queue_is_ordered_4_f_check_for_next_queued_duty(s_mod, s', dvn, n, index_next_attestation_duty_to_be_served);
+        } 
+        else 
+        {
+            lemma2_inv_attestation_duty_queue_is_ordered_4_body_body(dvn, n, process, s', index_next_attestation_duty_to_be_served);           
+        }     
+    }                 
+    
+    lemma lemma_inv_attestation_duty_queue_is_ordered_4_f_check_for_next_queued_duty(
+        process: DVCNodeState,
+        s': DVCNodeState,
+        dvn: DVState,
+        n: BLSPubkey,
+        index_next_attestation_duty_to_be_served: nat
+    )
+    requires f_check_for_next_queued_duty.requires(process)
+    requires s' == f_check_for_next_queued_duty(process).state  
+    requires inv_attestation_duty_queue_is_ordered_4_body_body(dvn, n, process, index_next_attestation_duty_to_be_served)  
+    ensures inv_attestation_duty_queue_is_ordered_4_body_body(dvn, n, s', index_next_attestation_duty_to_be_served)      
+    decreases process.attestation_duties_queue
+    {
+        if  && process.attestation_duties_queue != [] 
+            && (
+                || process.attestation_duties_queue[0].slot in process.future_att_consensus_instances_already_decided
+                || !process.current_attestation_duty.isPresent()
+            )    
+        {
+            if process.attestation_duties_queue[0].slot in process.future_att_consensus_instances_already_decided.Keys
+            {
+                var queue_head := process.attestation_duties_queue[0];
+                var new_attestation_slashing_db := f_update_attestation_slashing_db(process.attestation_slashing_db, process.future_att_consensus_instances_already_decided[queue_head.slot]);
+                var s_mod := process.(
+                    attestation_duties_queue := process.attestation_duties_queue[1..],
+                    future_att_consensus_instances_already_decided := process.future_att_consensus_instances_already_decided - {queue_head.slot},
+                    attestation_slashing_db := new_attestation_slashing_db,
+                    attestation_consensus_engine_state := updateConsensusInstanceValidityCheck(
+                        process.attestation_consensus_engine_state,
+                        new_attestation_slashing_db
+                    )                        
+                );
+
+                lemma3_inv_attestation_duty_queue_is_ordered_4_body_body(dvn, n, process, s_mod, index_next_attestation_duty_to_be_served);
+                lemma_inv_attestation_duty_queue_is_ordered_4_f_check_for_next_queued_duty(s_mod, s', dvn, n , index_next_attestation_duty_to_be_served);
+            }
+            else 
+            {
+                var new_process := process.(
+                    attestation_duties_queue := process.attestation_duties_queue[1..]
+                );   
+
+                var queue_head := process.attestation_duties_queue[0];      
+                lemma3_inv_attestation_duty_queue_is_ordered_4_body_body(dvn, n, process, new_process, index_next_attestation_duty_to_be_served);                 
+
+
+                // assert inv_g_a_ii_a_body_body(dvn, n, s');
+
+            }
+        } 
+        else 
+        {
+            lemma2_inv_attestation_duty_queue_is_ordered_4_body_body(dvn, n, process, s', index_next_attestation_duty_to_be_served);
+        }       
+    }     
+
+    lemma lemma_inv_attestation_duty_queue_is_ordered_4_honest(
+        s: DVState,
+        event: DV.Event,
+        s': DVState
+    )
+    requires NextEvent(s, event, s')   
+    requires 
+        && inv_attestation_duty_queue_is_ordered_3(s) //  
+        && inv_attestation_duty_queue_is_ordered_4(s) //  
+        && is_sequence_attestation_duties_to_be_served_orderd(s) //     
+    requires event.HonestNodeTakingStep?
+    ensures inv_attestation_duty_queue_is_ordered_4_body_body(s', event.node, s'.honest_nodes_states[event.node], s'.index_next_attestation_duty_to_be_served) 
+    {
+        assert s.att_network.allMessagesSent <= s'.att_network.allMessagesSent;
+        match event 
+        {
+            
+            case HonestNodeTakingStep(node, nodeEvent, nodeOutputs) =>
+                var s_node := s.honest_nodes_states[node];
+                var s'_node := s'.honest_nodes_states[node];
+
+                lemma_pred_4_1_b_new_helper_transpose_to_new_s_3(s, event, s', s_node, node);
+                lemma_inv_sequence_attestation_duties_to_be_served_orderd(s, event, s');
+
+                assert inv_attestation_duty_queue_is_ordered_4_body_body(s', node, s_node, s.index_next_attestation_duty_to_be_served);
+
+                match nodeEvent
+                {
+                    case ServeAttstationDuty(attestation_duty) => 
+                        assert s.index_next_attestation_duty_to_be_served == s'.index_next_attestation_duty_to_be_served - 1;
+                        lemma_ServeAttstationDuty(s, event, s');
+                        lemma_inv_attestation_duty_queue_is_ordered_4_f_serve_attestation_duty(
+                            s_node,
+                            attestation_duty,
+                            s'_node,
+                            s', 
+                            node,
+                            s'.index_next_attestation_duty_to_be_served
+                        );
+                        assert inv_attestation_duty_queue_is_ordered_4_body_body(s', node, s'_node, s'.index_next_attestation_duty_to_be_served);                     
+                
+                    case AttConsensusDecided(id, decided_attestation_data) =>  
+                        lemma_NonServeAttstationDuty(s, event, s');
+                        assert s.index_next_attestation_duty_to_be_served == s'.index_next_attestation_duty_to_be_served;    
+                        lemma_inv_attestation_duty_queue_is_ordered_4_f_att_consensus_decided(
+                            s_node,
+                            id,
+                            decided_attestation_data,
+                            s'_node,
+                            s', 
+                            node,
+                            s.index_next_attestation_duty_to_be_served
+                        ); 
+                        assert inv_attestation_duty_queue_is_ordered_4_body_body(s', node, s'_node, s'.index_next_attestation_duty_to_be_served);                        
+               
+                   
+                    case ReceviedAttesttionShare(attestation_share) =>
+                        lemma_NonServeAttstationDuty(s, event, s'); 
+                        lemma_f_listen_for_attestation_shares_constants(s_node, attestation_share, s'_node);
+                        lemma2_inv_attestation_duty_queue_is_ordered_4_body_body(s', node, s_node, s'_node, s'.index_next_attestation_duty_to_be_served);
+                        assert inv_attestation_duty_queue_is_ordered_4_body_body(s', node, s'_node, s'.index_next_attestation_duty_to_be_served);  
+                        
+
+                    case ImportedNewBlock(block) => 
+                        lemma_NonServeAttstationDuty(s, event, s');
+                        var s_node2 := add_block_to_bn(s_node, nodeEvent.block);
+                        lemma2_inv_attestation_duty_queue_is_ordered_4_body_body(s', node, s_node, s_node2, s'.index_next_attestation_duty_to_be_served);
+                        lemma_inv_attestation_duty_queue_is_ordered_4_f_listen_for_new_imported_blocks(
+                            s_node2,
+                            block,
+                            s'_node,
+                            s', 
+                            node,
+                            s.index_next_attestation_duty_to_be_served
+                        );  
+                        assert inv_attestation_duty_queue_is_ordered_4_body_body(s', node, s'_node, s'.index_next_attestation_duty_to_be_served);                     
+                    
+                 
+                    case ResendAttestationShares => 
+                        lemma_NonServeAttstationDuty(s, event, s');
+                        lemma_f_resend_attestation_share_constants(s_node, s'_node);
+                        lemma2_inv_attestation_duty_queue_is_ordered_4_body_body(s', node, s_node, s'_node, s'.index_next_attestation_duty_to_be_served);
+                        assert inv_attestation_duty_queue_is_ordered_4_body_body(s', node, s'_node, s'.index_next_attestation_duty_to_be_served); 
+
+                    case NoEvent => 
+                        lemma_NonServeAttstationDuty(s, event, s');
+                        assert s_node == s'_node; 
+                        lemma2_inv_attestation_duty_queue_is_ordered_4_body_body(s', node, s_node, s'_node, s'.index_next_attestation_duty_to_be_served);
+                        assert inv_attestation_duty_queue_is_ordered_4_body_body(s', node, s'_node, s'.index_next_attestation_duty_to_be_served);                          
+                }                
+        }
+    }   
+
+    lemma lemma_inv_attestation_duty_queue_is_ordered_4_helper_other_node(
+        s: DVState,
+        event: DV.Event,
+        s': DVState,
+        hn: BLSPubkey
+    )
+    requires NextEvent(s, event, s')
+    requires 
+        && inv_attestation_duty_queue_is_ordered_3(s) //  
+        && inv_attestation_duty_queue_is_ordered_4(s) //    
+        && is_sequence_attestation_duties_to_be_served_orderd(s) //     
+    requires event.HonestNodeTakingStep?
+    requires event.event.ServeAttstationDuty?
+    requires event.node != hn 
+    requires hn in s.honest_nodes_states
+    ensures inv_attestation_duty_queue_is_ordered_4_body_body(s', hn, s'.honest_nodes_states[hn], s'.index_next_attestation_duty_to_be_served)
+    {
+        lemma_pred_4_1_b_new_helper_transpose_to_new_s_3(s, event, s', s.honest_nodes_states[hn], hn);
+
+        assert s'.index_next_attestation_duty_to_be_served == s.index_next_attestation_duty_to_be_served + 1;
+
+        assert s.sequence_attestation_duties_to_be_served[s.index_next_attestation_duty_to_be_served].node == event.node;
+
+        var s_nodeh := s.honest_nodes_states[hn];
+        var s'_nodeh := s'.honest_nodes_states[hn];
+
+        assert inv_attestation_duty_queue_is_ordered_4_body_body(s', hn, s_nodeh, s.index_next_attestation_duty_to_be_served);
+
+        if |s'_nodeh.attestation_duties_queue| > 0
+        {
+            assert |s_nodeh.attestation_duties_queue| > 0;
+
+            forall i: nat |
+                inv_attestation_duty_queue_is_ordered_4_body_body_premise(
+                    s',
+                    hn, 
+                    s'_nodeh,
+                    i,
+                    s'.index_next_attestation_duty_to_be_served
+                )
+            ensures 
+                var last := seq_last(s'_nodeh.attestation_duties_queue);
+                last.slot == s'.sequence_attestation_duties_to_be_served[i].attestation_duty.slot;
+            {
+                var last := seq_last(s'_nodeh.attestation_duties_queue);
+
+                var lastp := seq_last(s_nodeh.attestation_duties_queue);
+
+                assert s.sequence_attestation_duties_to_be_served == s'.sequence_attestation_duties_to_be_served;
+
+                // assert last == lastp;
+
+                if i < s.index_next_attestation_duty_to_be_served
+                {
+                    assert 
+                        inv_attestation_duty_queue_is_ordered_4_body_body_premise(
+                            s',
+                            hn, 
+                            s_nodeh,
+                            i,
+                            s.index_next_attestation_duty_to_be_served
+                        );
+                    assert lastp.slot == s'.sequence_attestation_duties_to_be_served[i].attestation_duty.slot; 
+                    assert last == lastp;
+                }
+                else 
+                {
+                    assert i == s.index_next_attestation_duty_to_be_served;
+                    assert s.sequence_attestation_duties_to_be_served[i].node == event.node;
+                    assert i == s'.index_next_attestation_duty_to_be_served - 1;
+                    assert s'.sequence_attestation_duties_to_be_served[i].node == event.node;
+                    assert false;
+                }
+            }
+        }       
+    }       
+
+
+    lemma lemma_inv_attestation_duty_queue_is_ordered_4(
+        s: DVState,
+        event: DV.Event,
+        s': DVState
+    )
+    requires NextEvent(s, event, s')
+    requires 
+        && inv_attestation_duty_queue_is_ordered_3(s) //  
+        && inv_attestation_duty_queue_is_ordered_4(s) //    
+        && is_sequence_attestation_duties_to_be_served_orderd(s) //    
+    ensures inv_attestation_duty_queue_is_ordered_4(s');  
+    {
+        assert s.att_network.allMessagesSent <= s'.att_network.allMessagesSent;
+        match event 
+        {
+            
+            case HonestNodeTakingStep(node, nodeEvent, nodeOutputs) =>
+                lemma_inv_attestation_duty_queue_is_ordered_4_honest(s, event, s');
+                   
+                forall hn |
+                    && hn in s'.honest_nodes_states.Keys   
+                ensures inv_attestation_duty_queue_is_ordered_4_body_body(s', hn, s'.honest_nodes_states[hn], s'.index_next_attestation_duty_to_be_served); 
+                {
+                    if hn != node 
+                    {
+                        assert s.honest_nodes_states[hn] == s'.honest_nodes_states[hn];
+                        lemma_pred_4_1_b_new_helper_transpose_to_new_s_3(s, event, s', s.honest_nodes_states[hn], hn);
+                        if event.event.ServeAttstationDuty?
+                        {
+                            lemma_inv_attestation_duty_queue_is_ordered_4_helper_other_node(
+                                s,
+                                event,
+                                s',
+                                hn
+                            );
+                        }
+                        else
+                        {
+                            assert inv_attestation_duty_queue_is_ordered_4_body_body(s', hn, s'.honest_nodes_states[hn], s'.index_next_attestation_duty_to_be_served);    
+                        }
+                        
+                    }
+                }  
+                         
+            case AdeversaryTakingStep(node, new_attestation_share_sent, messagesReceivedByTheNode) =>
+                forall hn |
+                    && hn in s'.honest_nodes_states.Keys   
+                ensures inv_attestation_duty_queue_is_ordered_4_body_body(s', hn, s'.honest_nodes_states[hn], s'.index_next_attestation_duty_to_be_served); 
+                {
+                    assert s'.index_next_attestation_duty_to_be_served == s.index_next_attestation_duty_to_be_served;
+                    lemma_pred_4_1_b_new_helper_transpose_to_new_s_3(s, event, s', s.honest_nodes_states[hn], hn);
+                    lemma2_inv_attestation_duty_queue_is_ordered_4_body_body(s', hn, s.honest_nodes_states[hn], s'.honest_nodes_states[hn], s'.index_next_attestation_duty_to_be_served);
+                }  
+
+        }
+    }            
 
 }
